Introduce stack of blackholed variables

LaunchburySimpl.thy
@@ -2,12 +2,12 @@ theory LaunchburySimpl
 imports Terms Heap
 begin
 
-inductive reds :: "heap \<Rightarrow> exp \<Rightarrow> var list \<Rightarrow> heap \<Rightarrow> exp \<Rightarrow> bool" ("_ : _ \<Down>\<^bsub>_\<^esub> _ : _" [50,50,50,50] 50)
+inductive reds :: "heap \<Rightarrow> exp \<Rightarrow> var list \<Rightarrow> var list \<Rightarrow> heap \<Rightarrow> exp \<Rightarrow> bool" ("_ : _ \<Down>\<^bsub>_;_\<^esub> _ : _" [50,50,50,50] 50)
 where
-  Lambda: "\<Gamma> : (Lam [x]. e) \<Down>\<^bsub>L\<^esub> \<Gamma> : (Lam [x]. e)" 
- | Application: "\<lbrakk> atom y \<sharp> (\<Gamma>,e,x,L,\<Delta>,\<Theta>,z) ; \<Gamma> : e \<Down>\<^bsub>x#L\<^esub> \<Delta> : (Lam [y]. e') ; \<Delta> : e'[y ::= x] \<Down>\<^bsub>L\<^esub> \<Theta> : z\<rbrakk> \<Longrightarrow> \<Gamma> : App e x \<Down>\<^bsub>L\<^esub> \<Theta> : z" 
- | Variable: "\<lbrakk> (x,e) \<in> set \<Gamma>; \<Gamma> : e \<Down>\<^bsub>L\<^esub> \<Delta> : z \<rbrakk> \<Longrightarrow> \<Gamma> : Var x \<Down>\<^bsub>L\<^esub> \<Delta> : z"
- | Let: "set (bn as) \<sharp>* (\<Gamma>, L) \<Longrightarrow> asToHeap as @ \<Gamma> : body \<Down>\<^bsub>L\<^esub> \<Delta> : z \<Longrightarrow> \<Gamma> : Let as body \<Down>\<^bsub>L\<^esub> \<Delta> : z"
+  Lambda: "\<Gamma> : (Lam [x]. e) \<Down>\<^bsub>L;S\<^esub> \<Gamma> : (Lam [x]. e)" 
+ | Application: "\<lbrakk> atom y \<sharp> (\<Gamma>,e,x,L,\<Delta>,\<Theta>,z,S) ; \<Gamma> : e \<Down>\<^bsub>x#L;S\<^esub> \<Delta> : (Lam [y]. e') ; \<Delta> : e'[y ::= x] \<Down>\<^bsub>L;S\<^esub> \<Theta> : z\<rbrakk> \<Longrightarrow> \<Gamma> : App e x \<Down>\<^bsub>L;S\<^esub> \<Theta> : z" 
+ | Variable: "\<lbrakk> (x,e) \<in> set \<Gamma>; x \<notin> set S; \<Gamma> : e \<Down>\<^bsub>L;x#S\<^esub> \<Delta> : z \<rbrakk> \<Longrightarrow> \<Gamma> : Var x \<Down>\<^bsub>L;S\<^esub> \<Delta> : z"
+ | Let: "set (bn as) \<sharp>* (\<Gamma>, L) \<Longrightarrow> asToHeap as @ \<Gamma> : body \<Down>\<^bsub>L;S\<^esub> \<Delta> : z \<Longrightarrow> \<Gamma> : Let as body \<Down>\<^bsub>L;S\<^esub> \<Delta> : z"
 
 equivariance reds
 
@@ -22,21 +22,21 @@ apply (auto simp add: fresh_star_def fresh_Pair exp_assn.fresh)
 done
 
 lemma eval_test:
-  "[] : (Let (ACons x (Lam [y]. Var y) ANil) (Var x)) \<Down>\<^bsub>[]\<^esub> [(x, Lam [y]. Var y)] : (Lam [y]. Var y)"
+  "[] : (Let (ACons x (Lam [y]. Var y) ANil) (Var x)) \<Down>\<^bsub>[];[]\<^esub> [(x, Lam [y]. Var y)] : (Lam [y]. Var y)"
 apply(auto intro!: Lambda Application Variable Let
  simp add: fresh_Pair fresh_Cons fresh_Nil exp_assn.fresh fresh_star_def)
 done
 
 lemma eval_test2:
-  "y \<noteq> x \<Longrightarrow> [] : (Let (ACons x (Lam [y]. Var y) ANil) (App (Var x) x)) \<Down>\<^bsub>[]\<^esub> [(x, Lam [y]. Var y)] : (Lam [y]. Var y)"
+  "y \<noteq> x \<Longrightarrow> [] : (Let (ACons x (Lam [y]. Var y) ANil) (App (Var x) x)) \<Down>\<^bsub>[];[]\<^esub> [(x, Lam [y]. Var y)] : (Lam [y]. Var y)"
 by (auto intro!: Lambda Application Variable Let simp add: fresh_Pair fresh_at_base fresh_Cons fresh_Nil exp_assn.fresh fresh_star_def)
 
 lemma reds_doesnt_forget:
-  "\<Gamma> : e \<Down>\<^bsub>L\<^esub> \<Delta> : z \<Longrightarrow> heapVars \<Gamma> \<subseteq> heapVars \<Delta>"
+  "\<Gamma> : e \<Down>\<^bsub>L;S\<^esub> \<Delta> : z \<Longrightarrow> heapVars \<Gamma> \<subseteq> heapVars \<Delta>"
 by(induct rule: reds.induct, auto)
 
 lemma reds_avoids_live:
-  "\<lbrakk> \<Gamma> : e \<Down>\<^bsub>L\<^esub> \<Delta> : z;
+  "\<lbrakk> \<Gamma> : e \<Down>\<^bsub>L;[]\<^esub> \<Delta> : z;
    x \<in> set L;
    x \<notin> heapVars \<Gamma>
   \<rbrakk> \<Longrightarrow> x \<notin> heapVars \<Delta>"
@@ -61,13 +61,13 @@ case (Let as \<Gamma> L body \<Delta> z)
 qed
 
 
-lemma reds_fresh:" \<lbrakk> \<Gamma> : e \<Down>\<^bsub>L\<^esub> \<Delta> : z;
+lemma reds_fresh:" \<lbrakk> \<Gamma> : e \<Down>\<^bsub>L;[]\<^esub> \<Delta> : z;
    atom (x::var) \<sharp> (\<Gamma>, e)
   \<rbrakk> \<Longrightarrow> atom x \<sharp> (\<Delta>, z) \<or> x \<in> heapVars \<Delta>"
 proof(induct rule: reds.induct)
 case (Lambda \<Gamma> x e) thus ?case by auto
 next
-case (Application y \<Gamma> e x' L \<Delta> \<Theta> z e')
+case (Application y \<Gamma> e x' L \<Delta> \<Theta> z S e')
   hence "atom x \<sharp> (\<Delta>, Lam [y]. e') \<or> x \<in> heapVars \<Delta>" by (auto simp add: exp_assn.fresh fresh_Pair)
 
   thus ?case
@@ -93,10 +93,10 @@ case (Application y \<Gamma> e x' L \<Delta> \<Theta> z e')
   qed
 next
 
-case(Variable v e \<Gamma> L \<Delta> z)  
+case(Variable v e \<Gamma> S L \<Delta> z)  
   have "atom x \<sharp> \<Gamma>" and "atom x \<sharp> v" using Variable.prems(1) by (auto simp add: fresh_Pair exp_assn.fresh)
   hence "atom x \<sharp> \<Gamma>" and "atom x \<sharp> e" using `(v,e) \<in> set \<Gamma>` by(auto intro: fresh_remove dest:fresh_list_elem)
-  hence "atom x \<sharp> (\<Delta>, z) \<or> x \<in> heapVars \<Delta>"  using Variable.hyps(3) by (auto simp add: fresh_Pair)
+  hence "atom x \<sharp> (\<Delta>, z) \<or> x \<in> heapVars \<Delta>"  using Variable.hyps(4) by (auto simp add: fresh_Pair)
   thus ?case using `atom x \<sharp> v` by (auto simp add: fresh_Pair fresh_Cons fresh_at_base)
 next
 
